\begin{equation*}
    -i \hbar \frac{\mathrm{d}}{\mathrm{d}t} |\Psi(t)\rangle = \hat{H} |\Psi(t) \rangle
\end{equation*}

\begin{equation*}
    \commutator{x^{i}}{p^{j}} = i \hbar \delta^{ij}
\end{equation*}

\begin{equation*}
    \commutator{L^{i}}{L^{j}} = i\hbar \epsilon^{ijk}L^{k}
\end{equation*}

\begin{equation*}
    \hat{\vec{S}} = \frac{\hbar}{2} \vec{\sigma}
\end{equation*}

\begin{align*}
    \sigma_{x} &=
    \begin{pmatrix}
        0 & 1 \\
        1 & 0
    \end{pmatrix} \\
    \sigma_{y} &=
    \begin{pmatrix}
        0 & -i \\
        i & 0
    \end{pmatrix} \\
    \sigma_{z} &=
    \begin{pmatrix}
        1 & 0 \\
        0 & -1
    \end{pmatrix}
\end{align*}

\begin{equation*}
    \commutator{S^{i}}{S^{j}} = i\hbar \epsilon^{ijk}S^{k}
\end{equation*}

\begin{align*}
    \commutator{\vec{A} \vec{B}}{\vec{C}} &= \vec{A}\commutator{\vec{B}}{\vec{C}} + \commutator{\vec{A}}{\vec{B}}\vec{C} \\
    \commutator{\vec{A}}{\vec{B}\vec{C}} &= \commutator{\vec{A}}{\vec{B}}\vec{C} + \vec{B}\commutator{\vec{A}}{\vec{C}}
\end{align*}

\begin{equation*}
\end{equation*}


\begin{align*}
    E_{n}^{(1)} &= \langle E_{n}^{(0)} | H_{I} | E_{n}^{(0)} \rangle \\
    E_{n}^{(2)} &= \sum_{m \neq n} \langle E_{n}^{(0)} | H_{I} | E_{m}^{(0)} \rangle \frac{\langle E_{m}^{(0)} | H_{I} | E_{n}^{(0)} \rangle}{E_{n}^{(0)} - E_{m}^{(0)}} \\
\end{align*}
